eIris/proofmode/split.v
@@ -1,29 +1,28 @@
 From elpi Require Import elpi.
 From iris.proofmode Require Export tactics coq_tactics reduction.
 From iris.prelude Require Import options.
-From iris.heap_lang Require Import proofmode.
 
 From eIris.common Extra Dependency "stdpp.elpi" as stdpp.
 From eIris.proofmode.elpi Extra Dependency "iris_ltac.elpi" as iris_ltac.
 
 Elpi Tactic eiSplitL.
 
-Ltac helper_eiSplit HS := eapply tac_sep_split with Left HS _ _.
+Ltac helper_eiSplit SIDE HS := eapply tac_sep_split with SIDE HS _ _.
 
 (* TODO: Look at how to use refine instead of eapply here or in another tactic*)
 Elpi Accumulate File stdpp.
 Elpi Accumulate File iris_ltac.
 Elpi Accumulate lp:{{
-  type sep_split term -> open-tactic.
-    sep_split HS G GL :- coq.ltac.call "helper_eiSplit" [trm HS] G GL.
+  type sep_split term -> term -> open-tactic.
+    sep_split SIDE HS G GL :- coq.ltac.call "helper_eiSplit" [trm SIDE, trm HS] G GL.
 
-  solve (goal _Ctx _Trigger _Type _Proof [str HSS] as G) GL :-
+  solve (goal _Ctx _Trigger _Type _Proof [trm SIDE, str HSS] as G) GL :-
     rex.split " " HSS HS,
     std.map HS string->stringterm HTS,
     std.map HTS (x\ r\ r = {{ INamed lp:x }}) HI,
     list->listterm HI TI,
     coq.typecheck TI {{ list ident }} ok, % Fill in any holes created when contructing the term
-    sep_split TI G [G0, G1 | GL0],
+    sep_split SIDE TI G [G0, G1 | GL0],
     coq.ltac.open tc_solve G0 GL1,
     coq.ltac.open pm_reduce G1 [G3 | GL2],
     coq.ltac.open split G3 GL3,
@@ -32,4 +31,7 @@ Elpi Accumulate lp:{{
 Elpi Typecheck.
 
 Tactic Notation "eiSplitL" string(t) :=
-  elpi eiSplitL ltac_string:(t).
+  elpi eiSplitL (Left) ltac_string:(t).
+
+  Tactic Notation "eiSplitR" string(t) :=
+  elpi eiSplitL (Right) ltac_string:(t).
