eIris/proofmode/startProof.v
@@ -1,0 +1,74 @@
+From elpi Require Import elpi.
+From iris.proofmode Require Export tactics coq_tactics reduction.
+From iris.prelude Require Import options.
+
+From eIris.common Extra Dependency "stdpp.elpi" as stdpp.
+From eIris.proofmode.elpi Extra Dependency "iris_ltac.elpi" as iris_ltac.
+
+From eIris.proofmode Require Import split.
+
+From iris.heap_lang Require Import proofmode.
+ 
+Elpi Tactic eiStartProof.
+
+Elpi Accumulate File stdpp.
+Elpi Accumulate File iris_ltac.
+Elpi Accumulate lp:{{
+  pred refine.notypeclass i:term, i:goal, o:list sealed-goal.
+  refine.notypeclass T (goal _ RawEv Ty Ev _) GS :-
+    rm-evar RawEv Ev,
+    @no-tc! => @keepunivs! => coq.elaborate-skeleton T Ty TR ok,
+    coq.ltac.collect-goals TR GS _,
+    RawEv = T,
+    Ev = TR.
+
+  pred refine.unify o:term, i:goal, o:list sealed-goal.
+  refine.unify T (goal _ RawEv Ty Ev _) GS :-
+    coq.say "Pre rm-evar",
+    print_constraints,
+    rm-evar RawEv Ev, % rm-evar throws away the evar constraint on P, but doesn't affect the name of P.
+    coq.say "Post rm-evar",
+    print_constraints,
+    @keepunivs! => coq.elaborate-skeleton T Ty TR ok, % elaborate skeleton for some reason throws away the name of P and replaces it with elpi_ctx_entry_1_. 
+    coq.ltac.collect-goals TR GS _,
+    RawEv = T,
+    Ev = TR.
+
+  solve (goal _Ctx _Trigger {{ let _ := _ in _ }} _Proof [] as _G) _GL :- !,
+    coq.error "iStartProof: goal is a `let`, use `simpl`, `intros x`, `iIntros (x)`, or `iIntros ""%x""".
+
+  solve (goal _Ctx _Trigger {{ envs_entails _ _ }} _Proof [] as G) GL :- !,
+    GL = [seal G].
+
+  solve (goal _Ctx _Trigger Type _Proof [] as G) GL :- 
+    refine.notypeclass {{ as_emp_valid_2 lp:Type _ _ }} G [G1, G2 | GL0],
+    coq.ltac.open tc_solve G1 GL1,
+    % coq.sigma.print,
+    coq.ltac.open (refine.unify {{ tac_start _ _ }}) G2 GL2,
+    std.append GL0 { std.append GL1 GL2 } GL.
+    % coq.sigma.print.
+
+}}.
+Elpi Typecheck.
+
+Tactic Notation "eiStartProof" :=
+  elpi eiStartProof.
+
+Section proof. 
+  Context `{!heapGS Σ}.
+  Notation iProp := (iProp Σ).
+
+  Elpi Trace Browser.
+
+  Lemma and_exist_sep (P : iProp) :
+    P -∗ P.
+  Proof.
+    (* iStartProof.
+    Show Proof. *)
+    eiStartProof.
+    Show Proof.
+    iIntros.
+    Show Proof.
+  Qed.
+  
+End proof.
