eIris/tests/test_elpi.v
@@ -4,6 +4,12 @@ From iris.prelude Require Import options.
 From iris.heap_lang Require Import proofmode.
 From eIris.proofmode Require Import split.
 
+Elpi Tactic print_args.
+Elpi Accumulate lp:{{
+  solve (goal _ _ _ _ Args) _ :- coq.say Args.
+}}.
+Elpi Typecheck.
+
 Section proof. 
   Context `{!heapGS Σ}.
   Notation iProp := (iProp Σ).
